lib/Iteration.v
@@ -12,6 +12,7 @@
 
 (* Bounded and unbounded iterators *)
 
+Require Import Axioms.
 Require Import Coqlib.
 Require Import Classical.
 Require Import Max.
