Makefile
@@ -33,7 +33,7 @@ GPATH=$(DIRS)
 
 # General-purpose libraries (in lib/)
 
-LIB=Coqlib.v Intv.v Maps.v Lattice.v Ordered.v \
+LIB=Axioms.v Coqlib.v Intv.v Maps.v Lattice.v Ordered.v \
   Iteration.v Integers.v Floats.v Parmov.v UnionFind.v
 
 # Parts common to the front-ends and the back-end (in common/)
